Flapjack/Test/Allocator.lean
@@ -23,6 +23,16 @@ example :
       some [(1, 3), (0, 2)] := by
   exact wordAllocateVarsWithClashes_safe_example
 
+example :
+    wordInstVars (.arith (.addCarry 1 2 3 4 5)) = [3, 4, 5, 1, 2] := by
+  exact wordInstVars_addCarry
+
+example :
+    wordAllocateLinearInstructions
+      [.arith (.addCarry 0 1 2 3 4), .arith (.addCarry 5 6 0 1 2)] =
+      some { vars := [(6, 8), (5, 7), (1, 3), (0, 2), (4, 6), (3, 5), (2, 4)] } := by
+  exact wordAllocateLinearInstructions_example
+
 example (slots : List Nat) (edges : List (Nat × Nat))
     (colouring : NatInfoMap Nat)
     (hcolouring : wordAllocateVarsWithClashes slots edges = some colouring) :
